src/Lang.v
@@ -1,0 +1,60 @@
+Require Import
+  Hask.Control.Monad
+  Hask.Data.Either
+  Lib
+  Ty
+  Exp
+  Sub
+  Sem
+  Step.
+
+From Equations Require Import Equations.
+Set Equations With UIP.
+
+Section Lang.
+
+Generalizable All Variables.
+
+Import ListNotations.
+
+Context {A : Type}.
+Context `{S : HostExprsSem A}.
+
+Class HostLang (A : Type) : Type := {
+  has_host_exprs_sem :> HostExprsSem A;
+
+
+(*
+  CallHost_sound {Γ dom cod} (f : HostExp (dom ⟶ cod))
+                 (v : Exp Γ dom) (H : ValueP v) se :
+    (HostExpSem f >>= λ f', SemExp v se >>= λ x, f' x) =
+      SemExp (CallHost f v H) se;
+
+  CallHost_irr {Γ dom cod} (f : HostExp (dom ⟶ cod))
+               (v : Exp Γ dom) (H : ValueP v) :
+    ¬ (CallHost f v H = APP (HostedFun f) v);
+
+  CallHost_preserves_renaming {Γ Γ' dom cod} (f : HostExp (dom ⟶ cod))
+               (v : Exp Γ dom) (H : ValueP v) (σ : Ren Γ' Γ) :
+    APP (HostedFun f) (RenExp σ v) ---> RenExp σ (CallHost f v H);
+
+  CallHost_preserves_substitution {Γ Γ' dom cod} (f : HostExp (dom ⟶ cod))
+               (v : Exp Γ dom) (H : ValueP v) (σ : Sub Γ' Γ) :
+    APP (HostedFun f) (SubExp σ v) ---> SubExp σ (CallHost f v H);
+
+
+  Reduce_sound {Γ τ} (h : HostExp τ) se :
+    HostExpSem h = SemExp (projT1 (Reduce (Γ:=Γ) h)) se;
+
+  Reduce_irr {Γ τ} (h : HostExp τ) :
+    ¬ (projT1 (Reduce (Γ:=Γ) h) = HostedExp h);
+
+  Reduce_preserves_renaming {Γ Γ' τ} (h : HostExp τ) (σ : Ren Γ Γ') :
+    RenExp σ (HostedExp h) ---> RenExp σ (projT1 (Reduce h));
+
+  Reduce_preserves_substitution {Γ Γ' τ} (h : HostExp τ) (σ : Sub Γ Γ') :
+    SubExp σ (HostedExp h) ---> SubExp σ (projT1 (Reduce h));
+*)
+}.
+
+End Lang.
