src/Lib.v
@@ -1,0 +1,25 @@
+Require Export
+  Coq.Classes.Morphisms
+  Coq.Classes.RelationClasses
+  Coq.Lists.List
+  Coq.Logic.Classical
+  Coq.Logic.ProofIrrelevance
+  Coq.Program.Equality
+  Coq.Program.Program
+  Coq.Relations.Relation_Definitions
+  Coq.Sets.Ensembles
+  Coq.Sets.Finite_sets
+  Coq.Sets.Finite_sets_facts
+  Coq.Sets.Powerset_facts
+  Coq.Strings.String
+  Coq.Unicode.Utf8.
+
+From Equations Require Import Equations.
+Set Equations With UIP.
+
+Corollary sum_id {X Y : Type} (e : X + Y) :
+  match e with
+  | inl x => inl x
+  | inr y => inr y
+  end = e.
+Proof. now destruct e. Qed.
