src/Ltac.v
@@ -1,4 +1,4 @@
-Require Export
+Require Import
   Coq.Unicode.Utf8
   Coq.Program.Equality
   Coq.Program.Program.
