src/Pact.v
@@ -1,4 +1,4 @@
-Require Export
+Require Import
   Coq.ZArith.ZArith
   Ty
   Exp
