src/Sound.v
@@ -1,0 +1,90 @@
+Require Import
+  Lib
+  Ltac
+  Ty
+  Exp
+  Sub
+  Sem
+  Step
+  Lang.
+
+From Equations Require Import Equations.
+Set Equations With UIP.
+
+Section Sound.
+
+Generalizable All Variables.
+
+Import ListNotations.
+
+Context {A : Type}.
+Context `{S : HostLang A}.
+
+Theorem Step_sound {Γ τ} (e : Exp Γ τ) v :
+  e ---> v → SemExp e = SemExp v.
+Proof.
+  intros.
+  induction H; simpl; auto;
+  extensionality se;
+  rewrite ?IHStep, ?sum_id; auto.
+  (* - destruct (SemExp_ValueP _ se X) as [? H]. *)
+  (*   simpl; rewrite H; simpl. *)
+  (*   now rewrite sum_id. *)
+  (* - now erewrite <- Reduce_sound. *)
+  (* - destruct (SemExp_ValueP _ se X) as [? H]. *)
+  (*   now simpl; rewrite H. *)
+  (* - destruct (SemExp_ValueP _ se X) as [? H1]. *)
+  (*   destruct (SemExp_ValueP _ se X0) as [? H2]. *)
+  (*   now simpl; rewrite H1, H2. *)
+  (* - destruct (SemExp_ValueP _ se X) as [? H1]. *)
+  (*   destruct (SemExp_ValueP _ se X0) as [? H2]. *)
+  (*   now simpl; rewrite H1, H2. *)
+  (* - destruct (SemExp_ValueP _ se X) as [? H]. *)
+  (*   now simpl; rewrite H. *)
+  (* - destruct (SemExp_ValueP _ se X) as [? H1]. *)
+  (*   destruct (SemExp_ValueP _ se X0) as [? H2]. *)
+  (*   now simpl; rewrite H1, H2. *)
+  (* - destruct (SemExp_ValueP _ se X) as [? H1]. *)
+  (*   destruct (SemExp_ValueP _ se X0) as [? H2]. *)
+  (*   now simpl; rewrite H1, H2. *)
+  (* - destruct (SemExp_ValueP _ se X) as [? H1]. *)
+  (*   destruct (SemExp_ValueP _ se X0) as [? H2]. *)
+  (*   now simpl; rewrite H1, H2. *)
+  (* - now apply CallHost_sound. *)
+  (* - destruct (SemExp_ValueP _ se X) as [? H1]. *)
+  (*   rewrite H1; simpl. *)
+  (*   rewrite sum_id. *)
+  (*   now erewrite <- SemExp_SubExp. *)
+  - admit.
+    (* rewrite <- SemExp_SubSem. *)
+    (* f_equal; simpl. *)
+    (* simp SubSem. *)
+    (* now rewrite SubSem_idSub. *)
+  (* - destruct (SemExp_ValueP _ se X) as [? H1]. *)
+  (*   now rewrite H1. *)
+Abort.
+
+(*
+Lemma If_loop_true {Γ τ} b {x : Exp Γ τ} {y : Exp Γ τ} :
+  ¬ (If b x y = x).
+Proof.
+  induction x; intro; inv H.
+  now eapply IHx2; eauto.
+Qed.
+
+Lemma If_loop_false {Γ τ} b {x : Exp Γ τ} {y : Exp Γ τ} :
+  ¬ (If b x y = y).
+Proof.
+  induction y; intro; inv H.
+  now eapply IHy3; eauto.
+Qed.
+
+Lemma Seq_loop {Γ τ ty} {x : Exp Γ ty} {y : Exp Γ τ} :
+  ¬ (Seq x y = y).
+Proof.
+  induction y; intro; inv H.
+  now eapply IHy2; eauto.
+Qed.
+*)
+
+End Sound.
